\documentclass[11pt]{article}
\usepackage{CJK}
\usepackage{amssymb}
\usepackage{latexsym}

\begin{document}
\begin{CJK}{GBK}{song}

\title{Homework 03 }
\author{ WISE ¸ßÇì»Ô 27720161153011 }

\maketitle

\begin{itemize}
\item 3.15 ANS:

From the PDF of X, we know that X has a continuous distribution $F_X(X)$ which is strictly monotonically increasing (when $1< x <3$).

So we can forms a 1-1 correspondence between $\mathbb{R}$ and interval $(0,1)$. Inverse function $F_X^{-1}(\cdot)$ exists and

\[ F_X(F_X^{-1}(y)) = y \]

for any $y \in \mathbb{R}$.

For $0<y<1$,

\begin{eqnarray*}
F_Y(y)=&P(F_X(X) \leq y)\\
=& P(X \leq F_X^{-1}(y))\\
=& F_X(F_X^{-1}(y))\mbox{}\\
=& y
\end{eqnarray*}

\[
f_Y(y)=\left\{
    \begin{array}{ll}
    1 &\mbox{$0<y<1$,}\\
    0 &\mbox{otherwise.}
    \end{array}
    \right.
\]

So Y follows Uniform $(0,1)$ distribution.

Calculate the CDF of X, we have

\[
F_X(X)=\left\{
    \begin{array}{ll}
    0 &\mbox{$x \le 1,$}\\
    \frac{(X-1)^2}{4}&\mbox{$1<x<3$,}\\
    1 &\mbox{$x \geq 3$.}
    \end{array}
    \right.
\]

so $Y=u(X)=F_X(X)$ follows Uniform$(0,1)$ distribution.



\item 3.23

The CDF of Y is
\begin{eqnarray*}
F_Y(y)=&P(Y \leq y)\\
=& P(X \leq F_X^{-1}(y))\\
=& F_X(F_X^{-1}(y))\mbox{}\\
=& y
\end{eqnarray*}


The CDF of Y is:

\begin{eqnarray*}
F_Y(y)=&P(Y \le y)\\
=&P(Y \le y | a < X) + P(Y \le y| a \le X \le b) + P(Y \le y | X < b)
\end{eqnarray*}

Since $\{a < X, a \le X \le b, X < b\}$ is a partition of S.

From $Y = X \cdot \mathbf{1} (a \le X \le b) $, we have

\begin{eqnarray*}
F_Y(y)=&P(Y \le y)\\
=&P(Y \le y | a < X) + P(Y \le y| a \le X \le b) + P(Y \le y | X < b)\\
=&P(X \le y| a \le X \le b) + P(X \le y | X < b) + P(X \le y | a < X)\\
=&P(X \le y| a \le X \le b) + P(X \le y | X < b) + P(X \le y | a < X)\\
=&\frac{P((X \le y) \cap (a \le X \le b)  )}{P((a \le X \le b))} + \frac{P((0 \le y) \cap (a < X)  )}{P(a < X)} + \frac{P((0 \le y) \cap (X < b))  }{P(X < b)}\\
=&\frac{P((X \le y) \cap (a \le X \le b)  )}{P((a \le X \le b))}\\
\end{eqnarray*}

Since $P((0 \le y) \cap (X < b)) = P((0 \le y) \cap (a < X))=0$.

So,
\begin{eqnarray*}
F_Y(y)=&\frac{P((X \le y) \cap (a \le X \le b)  )}{P(a \le X \le b)}& \\
=&\frac{F_X(y)}{F_X(b) - F_X(a)} & (a \le y \le b)
\end{eqnarray*}

we have

\begin{eqnarray*}
f_Y(y)=&F_Y'(y)& \\
=&\frac{f_X(y)}{F_X(b) - F_X(a)} & (a \le y \le b)
\end{eqnarray*}

\item 3.25 ANS:

\item 3.28 ANS:



\item 3.30 ANS:

a.

\[
\int_0^m 3x^2dx = m^3 = \frac{1}{2}
\]

so, $m = \frac{1}{2}^{1/3} = 0.794$

b.

The function is symmetric about zero, therefore m = 0 as long as the integral is finite.

\[ 
\frac{1}{\pi} \int_{-\infty}^{\infty} \frac{1}{1+x^2}dx = \frac{1}{\pi}tan^{-1}\arrowvert_{-\infty}^{\infty}=\frac{1}{\pi}(\frac{\pi}{2}+\frac{\pi}{2})=1
\]

\end{itemize} 

\end{CJK}
\end{document}
